Closer to having everything fully working

src/Types.fst
@@ -1,3 +1,0 @@
-module Types
-
-type state = int -> Tot bool
